Prove DRF-PROMISES (WIP)

src/lang/Event.v
@@ -92,4 +92,18 @@ Module ProgramEvent.
   | fence (ordr ordw:Ordering.t)
   | syscall (e:Event.t)
   .
+
+  Definition is_reading (e:t): option (Loc.t * Ordering.t) :=
+    match e with
+    | read loc _ ord => Some (loc, ord)
+    | update loc _ _ ordr _ => Some (loc, ordr)
+    | _ => None
+    end.
+
+  Definition is_writing (e:t): option (Loc.t * Ordering.t) :=
+    match e with
+    | write loc _ ord => Some (loc, ord)
+    | update loc _ _ _ ordw => Some (loc, ordw)
+    | _ => None
+    end.
 End ProgramEvent.
